Proved the property in Section 3.2 for the full Vellvm, which is the key property to prove transformation correctness. Note that the property only holds for 'pure' instructions. 'pure' instructions exclude memory operators---load/store/malloc/alloca/free/call, and operators that may cause non-derministic behavior---gep/select. In the deterministic version of Vellvm, gep/select is also pure.
git-svn-id: https://webdav.seas.upenn.edu/svn/sol/vol@3295 eef5ea85-cc2e-0410-bd84-0fae1f012da8

src/Vellvm/analysis.v
@@ -1019,8 +1019,7 @@ Definition inscope_of_block (f:fdef) (l1:l) (opt_ctx:option (list atom)) (lbl:l)
   | None => None
   end.
 
-Definition inscope_of_cmd (f:fdef) (b1:block) (c:cmd) : option (list atom) :=
-let id0 := getCmdLoc c in
+Definition inscope_of_id (f:fdef) (b1:block) (id0:id) : option (list atom) :=
 let '(block_intro l1 ps cs _) := b1 in
 let '(fdef_intro (fheader_intro _ _ _ la _) _) := f in
 let 'dt := dom_analyze f in
@@ -1028,6 +1027,9 @@ let '(Dominators.mkBoundedSet els _) := AMap.get l1 dt in
 fold_left (inscope_of_block f l1) els
   (Some (getPhiNodesIDs ps ++ cmds_dominates_cmd cs id0 ++ getArgsIDs la))
 .
+
+Definition inscope_of_cmd (f:fdef) (b1:block) (c:cmd) : option (list atom) :=
+let id0 := getCmdLoc c in inscope_of_id f b1 id0.
 
 Definition inscope_of_tmn (f:fdef) (b1:block) (tmn:terminator) 
   : option (list atom) :=
@@ -1181,7 +1183,7 @@ exists ids2,
   end.
 Proof.
   intros f l2 ps2 cs2' c' tmn' ids1 Hnotin Hinscope.
-  unfold inscope_of_cmd in Hinscope.
+  unfold inscope_of_cmd, inscope_of_id in Hinscope.
   unfold inscope_of_tmn.
   destruct f as [[? ? ? la va] bs].
   remember ((dom_analyze (fdef_intro (fheader_intro f t i0 la va) bs)) !! l2) as R.
@@ -1274,8 +1276,8 @@ exists ids2,
   end.
 Proof.
   intros f l2 ps2 cs2' c' c cs' tmn' ids1 Hnodup Hinscope.
-  unfold inscope_of_cmd in Hinscope.
-  unfold inscope_of_cmd.
+  unfold inscope_of_cmd, inscope_of_id in Hinscope.
+  unfold inscope_of_cmd, inscope_of_id.
   destruct f as [[? ? ? la va] bs].
   remember ((dom_analyze (fdef_intro (fheader_intro f t i0 la va) bs)) !! l2) as R.
   destruct R as [R_contents R_bound].
@@ -1338,14 +1340,12 @@ Proof.
       contradict n; auto.
 Qed.
 
-Lemma fold_left__bound_blocks : forall ls0 fa t i0 la va bs l0 init,
+Lemma fold_left__bound_blocks : forall ls0 fh bs l0 init,
   incl ls0 (bound_blocks bs) ->
   exists r, 
-    fold_left (inscope_of_block 
-      (fdef_intro (fheader_intro fa t i0 la va) bs) l0) ls0 (Some init) = 
-       Some r.
+    fold_left (inscope_of_block (fdef_intro fh bs) l0) ls0 (Some init) = Some r.
 Proof.
-  induction ls0; intros fa t i0 la va bs l0 init Hinc; simpl in *.
+  induction ls0; intros fh bs l0 init Hinc; simpl in *.
     exists init. auto.
 
     assert (incl ls0 (bound_blocks bs)) as J.
